Progtess on terms! Documentation generation! Proper Makefile! README!

definitions/terms.v
@@ -1,7 +1,37 @@
+(** * Terms
+
+    In this file, System-T terms are defined, with a few base notions
+    related to them (closedness, substitutions).
+*)
+
+Require Import Nat.
+Require Import Logic.Decidable.
+Require Import Coq.Arith.Compare_dec.
+
 Declare Scope system_t_term_scope.
 
+(** ** Terms
+*)
+
+(** [idenT] is the label type for free variables.
+*)
+Definition identT := nat.
+
+(** [termT] is the [Type] representing the terms of System-T.
+
+    Free variables are distinguished from bound variables, to avoid
+    alpha-conversion issues.
+
+    Free variables are labeled with [identT] values.
+
+    Bound variables are represented by de Bruijn indexes. Because of
+    that, a [termT] may correspond to something that is not a real
+    System-T term, because some of its bound variables may be bound to
+    nonexistant lambdas.
+*)
 Inductive termT :=
-  | xT : nat -> termT
+  | fvarT : identT -> termT
+  | bvarT : nat -> termT
   | absT : termT -> termT
   | appT : termT -> termT -> termT
   | oT : termT
@@ -10,3 +40,146 @@ Inductive termT :=
   | falseT : termT
   | iteT : termT -> termT -> termT -> termT
   | recT : termT -> termT -> termT -> termT.
+
+(** ** Closedness : Definitions
+*)
+
+(** A [termT] is [bound_nclosed n] when all its de Bruijn indexes
+    refer to lambdas that are at height at most [n] above its root.
+
+    Obviously, the good notion of closedness is [bound_nclosed O],
+    as it states that all bound variables are bound to lambdas
+    actually within the term, but we use a depth-dependent version
+    as it is needed for the inductive structure. 
+*)
+Inductive bound_nclosed : nat -> termT -> Prop :=
+  | fvarT_closed :
+    forall n : nat, forall x : identT,
+    bound_nclosed n (fvarT x)
+  | bvarT_closed :
+    forall n x : nat, x <= n ->
+    bound_nclosed n (bvarT x)
+  | absT_closed :
+    forall n : nat, forall u : termT,
+    bound_nclosed (S n) u ->
+    bound_nclosed n (absT u)
+  | appT_closed :
+    forall n : nat, forall u v : termT,
+    bound_nclosed n u ->
+    bound_nclosed n v ->
+    bound_nclosed n (appT u v)
+  | oT_closed :
+    forall n : nat, bound_nclosed n oT
+  | sT_closed :
+    forall n : nat, forall u : termT,
+    bound_nclosed n u ->
+    bound_nclosed n (sT u)
+  | trueT_closed :
+    forall n : nat, bound_nclosed n trueT
+  | falseT_closed :
+    forall n : nat, bound_nclosed n falseT
+  | iteT_closed :
+    forall n : nat, forall u v w : termT,
+    bound_nclosed n u ->
+    bound_nclosed n v ->
+    bound_nclosed n w ->
+    bound_nclosed n (iteT u v w)
+  | recT_closed :
+    forall n : nat, forall u v w : termT,
+    bound_nclosed n u ->
+    bound_nclosed n v ->
+    bound_nclosed n w ->
+    bound_nclosed n (recT u v w).
+
+(** ** Closedness : Decidability
+*)
+
+(** A [termT] is [bound_closed] when all its bound variables are
+    bound to lambdas actually within the term.
+*)
+Definition bound_closed := bound_nclosed O.
+
+(** [bound_nclosed n] is a decidable predicate for all [n].
+*)
+Lemma bound_nclosed_decidable (u : termT) :
+    forall n : nat, decidable (bound_nclosed n u).
+Proof.
+  induction u;
+  intro m;
+  [ |
+    destruct (dec_le n m) |
+    destruct (IHu (S m)) |
+    destruct (IHu1 m); destruct (IHu2 m) | |
+    destruct (IHu m) | | |
+    destruct (IHu1 m); destruct (IHu2 m); destruct (IHu3 m) |
+    destruct (IHu1 m); destruct (IHu2 m); destruct (IHu3 m)
+  ];
+    try (left; auto using bound_nclosed; fail);
+    right; intro Hn; inversion Hn; auto using bound_nclosed.
+Qed.
+
+(** [bound_closed n] is a decidable predicate.
+*)
+Lemma bound_closed_decidable (u : termT) :
+    decidable (bound_closed u).
+Proof.
+  exact (bound_nclosed_decidable u O).
+Qed.
+
+(** ** Substitutions
+*)
+
+(** [subst_bvarT n u a] is [u], where all the occurrences of the
+    variable bound by the lambda at height [n] above the root are
+    replaced by [a].
+*)
+Fixpoint subst_bvarT (n : nat) (u a : termT) :=
+  match u with
+  | bvarT m => 
+    match n =? m with
+    | true => a
+    | false => bvarT m
+    end
+  | absT u => absT (subst_bvarT (S n) u a)
+  | appT u v =>
+    appT (subst_bvarT n u a) (subst_bvarT n v a)
+  | sT u => sT (subst_bvarT n u a)
+  | iteT u v w =>
+    iteT
+      (subst_bvarT n u a)
+      (subst_bvarT n v a)
+      (subst_bvarT n w a)
+  | recT u v w =>
+    recT
+      (subst_bvarT n u a)
+      (subst_bvarT n v a)
+      (subst_bvarT n w a)
+  | _ => u
+  end.
+
+(** [subst_fvarT x u a] is [u], where all the occurrences of the
+    free variable labeled by [x] are replaced by [a].
+*)
+Fixpoint subst_fvarT (x : identT) (u a : termT) :=
+  match u with
+  | fvarT y => 
+    match x =? y with
+    | true => a
+    | false => bvarT y
+    end
+  | absT u => absT (subst_fvarT x u a)
+  | appT u v =>
+    appT (subst_fvarT x u a) (subst_fvarT x v a)
+  | sT u => sT (subst_fvarT x u a)
+  | iteT u v w =>
+    iteT
+      (subst_fvarT x u a)
+      (subst_fvarT x v a)
+      (subst_fvarT x w a)
+  | recT u v w =>
+    recT
+      (subst_fvarT x u a)
+      (subst_fvarT x v a)
+      (subst_fvarT x w a)
+  | _ => u
+  end.
