definitions/types.v
@@ -1,9 +1,9 @@
 Declare Scope system_t_type_scope.
 
-Inductive TypeT :=
-  | natT : TypeT
-  | boolT : TypeT
-  | tT : nat -> TypeT
-  | funT : TypeT -> TypeT -> TypeT.
+Inductive typeT :=
+  | natT : typeT
+  | boolT : typeT
+  | tT : nat -> typeT
+  | funT : typeT -> typeT -> typeT.
 
 Notation "t ->T u" := (funT t u) (at level 80, right associativity).
