definitions/typing.v
@@ -1,1 +1,26 @@
 Require Import types.
+Require Import terms.
+Require Import FSets.FMaps.
+
+Open Scope system_t_type_scope.
+Open Scope system_t_term_scope.
+
+Module FMap := FMapPositive.PositiveMap.
+
+Definition context := FMap.t typeT.
+
+Print context.
+
+(* Inductive typing_derivation : context -> termT -> typeT -> Type :=
+  | var :
+    forall G, forall n, forall t, G n = Some t ->
+    TypingDerivation G (xT n) t
+  | oTnatT :
+    forall G, TypingDerivation G oT natT
+  | sTnatT :
+    forall G, forall e, TypingDerivation G e natT ->
+    TypingDerivation G (sT e) natT. 
+*)
+
+Close Scope system_t_type_scope.
+Close Scope system_t_term_scope.
