Makefile
@@ -1,0 +1,37 @@
+KNOWNTARGETS 			:= CoqMakefile
+KNOWNFILES   			:= Makefile _CoqProject
+DEFINITIONS_FILES := definitions/*.v
+
+.DEFAULT_GOAL := invoke-coqmakefile
+
+CoqMakefile: Makefile _CoqProject
+				$(COQBIN)coq_makefile -f _CoqProject -o CoqMakefile
+
+invoke-coqmakefile: CoqMakefile
+				$(MAKE) --no-print-directory -f CoqMakefile $(filter-out $(KNOWNTARGETS),$(MAKECMDGOALS))
+
+create-doc-folder:
+				@echo "Creating documentation directory."
+
+				@mkdir -p documentation
+
+build-doc: | create-doc-folder
+				@echo "Building documentation."
+				@for f in definitions/*.v; do \
+						echo "Building documentation for file $${f}."; \
+						coqdoc -d documentation $${f}; \
+				done
+				
+
+clean:
+				@echo "Deleting build files."
+				@rm -rf definitions/*.vo definitions/*.vok definitions/*.vos definitions/*.glob definitions/.*.aux
+				@echo "Deleting documentation."
+				@rm -rf documentation
+
+all: invoke-coq_makefile build-doc
+
+.PHONY: invoke-coqmakefile $(KNOWNFILES)
+
+%: invoke-coqmakefile
+				@true
