README.md
@@ -1,0 +1,35 @@
+# System-T
+
+## Overview
+
+An attempt to formalize Gödel's System-T using the _Coq_ (_Rocq_?) proof assistant, for **Alexis Saurin**'s _Functional Programming and Formal Proofs in Coq_ course at LMFI.
+
+In particular, the main goal of this project is to prove strong normalization for System-T.
+
+## Building the project
+
+- To build all _Coq_ files, run
+
+  ```{bash}
+  make
+  ```
+
+- To build documentation, run
+
+  ```{bash}
+  make build-doc
+  ```
+
+  A `documentation` directory will then be created with `html` formatted versions of the source files.
+
+- To do build both source files and documentation, run
+
+  ```{bash}
+  make all
+  ```
+
+- To delete all build files, run
+
+  ```{bash}
+  make clean
+  ```
